test/method_decls.thy
@@ -1,0 +1,68 @@
+theory method_decls
+ imports ViperCommon.ViperLang
+begin
+definition foo_body :: "((stmt) option)" where 
+  "foo_body  = (Some (Inhale (Atomic (AccPredicate ''P'' [(ViperLang.Var 0)] (PureExp (ELit WritePerm))))))"
+
+
+abbreviation foo_args :: "(((nat\<times>vtyp)) list)" where 
+  "foo_args  \<equiv> [(0,ViperLang.TRef)]"
+
+
+abbreviation foo_returns :: "(((nat\<times>vtyp)) list)" where 
+  "foo_returns  \<equiv> []"
+
+
+definition foo_pre where 
+  "foo_pre  = (Atomic (Pure (ELit (LBool True))))"
+
+
+definition foo_post where 
+  "foo_post  = (Atomic (Pure (ELit (LBool True))))"
+
+
+definition foo_decl where 
+  "foo_decl  = (method_decl.make [ViperLang.TRef] [] foo_pre foo_post foo_body)"
+
+
+lemma foo_decl_proj_margs : 
+
+shows "((method_decl.args foo_decl)=[ViperLang.TRef])"
+by (simp add: foo_decl_def method_decl.defs(1))
+
+
+lemma foo_decl_proj_mrets : 
+
+shows "((method_decl.rets foo_decl)=[])"
+by (simp add: foo_decl_def method_decl.defs(1))
+
+
+lemma foo_decl_proj_mpre : 
+
+shows "((method_decl.pre foo_decl)=(Atomic (Pure (ELit (LBool True)))))"
+by (simp add: foo_decl_def method_decl.defs(1) foo_pre_def)
+
+
+lemma foo_decl_proj_mpost : 
+
+shows "((method_decl.post foo_decl)=(Atomic (Pure (ELit (LBool True)))))"
+by (simp add: foo_decl_def method_decl.defs(1) foo_post_def)
+
+
+lemma foo_decl_proj_mbody : 
+
+shows "((method_decl.body foo_decl)=(Some (Inhale (Atomic (AccPredicate ''P'' [(ViperLang.Var 0)] (PureExp (ELit WritePerm)))))))"
+by (simp add: foo_decl_def method_decl.defs(1) foo_body_def)
+
+
+definition methodLookupFun where 
+  "methodLookupFun  = (map_of [(''foo'',method_decls.foo_decl)])"
+
+
+lemma foo_lookup_lemma : 
+
+shows "((methodLookupFun ''foo'')=(Some method_decls.foo_decl))"
+by (simp add: methodLookupFun_def)
+
+
+end
